notes.md
@@ -1,3 +1,7 @@
+- Syntax -> Name : getId
+- Name -> Syntax ?
+
+
 # Ideas
  - Make the tactics have a separate auxiliary function to return the actual proof term
    so we don't have to use evalTactic and keep refreshing the context
@@ -7,3 +11,5 @@
 # TODO
  - factoring tactic (remove duplicates in or-chain)
  - fix bug in resolution (if the resolvant itself is an Or)
+ - rewrite everything using option 2 from Wojciech (manipulate
+   syntax instead of expr)
